Inverted Index Search Terms.

src/QueryStructure/Implementation/DataStructures/BagADT/IndexSearchTerms.v
@@ -17,15 +17,112 @@ Require Import
 
 (* Implements a Search Term for heading as a list of optional key
    values given a list of attributes. *)
-Fixpoint BuildIndexSearchTerm {heading : Heading}
+
+Class IndexDenotation
+      (A : Set)
+      (heading : Heading)
+      (index : Attributes heading)
+  := { DenoteIndex : Type;
+       MatchIndex : DenoteIndex -> @Tuple heading -> bool
+  }.
+
+Inductive EqualityIndex : Set := equalityIndex.
+
+Global Instance EqualityIndexDenotation
+       (heading : Heading)
+       (index : Attributes heading)
+       (_ : Query_eq (Domain heading index))
+: @IndexDenotation EqualityIndex heading index :=
+  {| DenoteIndex :=
+       option (Domain heading index);
+     MatchIndex search_term tup :=
+       match search_term with
+         | Some val => if A_eq_dec (GetAttribute tup index) val then
+                         true
+                       else false
+         | _ => true
+       end
+  |}.
+
+Inductive UnIndex : Set := unIndex.
+Global Instance UnIndexDenotation
+       (heading : Heading)
+       (index : Attributes heading)
+: @IndexDenotation UnIndex heading index :=
+  {| DenoteIndex := @Tuple heading -> bool;
+     MatchIndex search_term tup := search_term tup
+  |}.
+
+Ltac BuildIndexSearchTerm'
+     attrs heading indices k :=
+  match indices with
+    | [(?kind, ?idx)] =>
+      k (@DenoteIndex kind heading (@Build_BoundedIndex _ attrs idx _) _)
+    | (?kind, ?idx) :: ?indices' =>
+      BuildIndexSearchTerm' attrs heading indices'
+                           ltac:(fun st' =>
+                                   k (prod (@DenoteIndex kind heading
+                                                         (@Build_BoundedIndex _ attrs idx _)  _) st'))
+  end.
+
+Ltac BuildIndexMatcher'
+     attrs heading indices k :=
+  match indices with
+    | [(?kind, ?idx)] =>
+      let idx' := constr:(@Build_BoundedIndex _ attrs idx _) in
+      k (@MatchIndex kind heading idx' _)
+    | (?kind, ?idx) :: ?indices' =>
+      let idx' := constr:(@Build_BoundedIndex _ attrs idx _) in
+      BuildIndexMatcher' attrs
+        heading indices'
+        ltac:(fun matcher' =>
+                k (fun st tup => (@MatchIndex kind heading idx' _ (fst st) tup)
+                               && matcher' (snd st) tup))
+  end.
+
+Record KindIndex
+       {heading : Heading}
+  := { KindIndexKind : Set;
+       KindIndexIndex : @Attributes heading }.
+
+Ltac BuildIndexes
+     attrs heading indices k :=
+  match indices with
+    | [(?kind, ?idx)] =>
+      let idx' := constr:(@Build_BoundedIndex _ attrs idx _) in
+      k ([@Build_KindIndex heading kind idx'])
+    | (?kind, ?idx) :: ?indices' =>
+      let idx' := constr:(@Build_BoundedIndex _ attrs idx _) in
+      BuildIndexes attrs
+                   heading indices'
+                   ltac:(fun indices'' =>
+                           k ((@Build_KindIndex heading kind idx') :: indices''))
+  end.
+
+(* Aliases to make existing automation happy. *)
+Definition BuildIndexSearchTerm
+           {heading : Heading}
+           (indices : list (@KindIndex heading))
+           {BuildIndexSearchTermT : Type}
+: Type := BuildIndexSearchTermT.
+
+Definition MatchIndexSearchTerm
+           {heading : Heading}
+           {indices : list (@KindIndex heading)}
+           {IndexSearchTermT : Type}
+           {matcher : IndexSearchTermT -> @Tuple heading -> bool} :
+  @BuildIndexSearchTerm heading indices IndexSearchTermT
+  -> @Tuple heading -> bool := matcher.
+
+(*Fixpoint BuildIndexSearchTerm {heading : Heading}
          (indices : list (@Attributes heading))
 : Type :=
   match indices with
     | [] => (@Tuple heading -> bool)
     | idx :: indices' => prod (option (Domain heading idx)) (BuildIndexSearchTerm indices')
-  end.
+  end. *)
 
-(* Implements a matcher function for a search term built using [BuildSearchTerm]. *)
+(* Implements a matcher function for a search term built using [BuildSearchTerm].
 Fixpoint MatchIndexSearchTerm {heading}
          {indices : list (@Attributes heading)}
          {eq_dec_indices : ilist (fun attr => Query_eq (Domain heading attr)) indices}
@@ -49,7 +146,7 @@ Fixpoint MatchIndexSearchTerm {heading}
                   && (H index' tup)
               | (None, index') => H index' tup
             end) (@MatchIndexSearchTerm _ _ (ilist_tl eq_dec_indices))
-  end eq_dec_indices.
+  end eq_dec_indices. *)
 
 Tactic Notation "build" "single" "index":=
 repeat match goal with
@@ -61,7 +158,7 @@ repeat match goal with
            simpl sch
        end.
 
-Ltac build_index_list heading As k :=
+(* Ltac build_index_list heading As k :=
   match As with
     | nil => k (inil (fun attr : Attributes heading => Query_eq (Domain heading attr)))
     | cons ?a ?As' =>
@@ -73,22 +170,27 @@ Ltac build_index_list heading As k :=
                                     a
                                     (_ : Query_eq (Domain heading a))
                                     Bs'))
-  end.
+  end. *)
 
 Ltac makeIndex' NamedSchemas IndexKeys k :=
   match NamedSchemas  with
     | nil => k (inil (fun ns : NamedSchema => SearchUpdateTerms (schemaHeading (relSchema ns))))
     | cons ?ns ?NamedSchemas' =>
       match IndexKeys with
-          | cons ?ik ?IndexKeys' =>
-            build_index_list (schemaHeading (relSchema ns)) ik
-                             ltac:(fun st =>
-                                     makeIndex' NamedSchemas' IndexKeys'
-                                                   ltac:(fun Bs' => k (icons ns
-                                                                             {| BagMatchSearchTerm := @MatchIndexSearchTerm _ _ st;
-                                                                                BagApplyUpdateTerm := fun z => z |} Bs')))
-      end
-  end.
+        | cons ?ik ?IndexKeys' =>
+          let attrs := eval simpl in (map attrName (AttrList (schemaHeading (relSchema ns)))) in
+              BuildIndexes attrs (schemaHeading (relSchema ns)) ik
+                           ltac:(fun attrs' =>
+                                   BuildIndexMatcher' attrs (schemaHeading (relSchema ns)) ik
+                                                      ltac:(fun matcher' =>
+                                                              makeIndex' NamedSchemas' IndexKeys'
+                                                                         ltac:(fun Bs' => k (icons ns
+                                                                                                   {| BagMatchSearchTerm := @MatchIndexSearchTerm
+                                                                                                                              (schemaHeading (relSchema ns)) attrs' _
+                                                                                                                              matcher';
+                                                                                                      BagApplyUpdateTerm := fun z => z |} Bs'))))
+                                 end
+                                 end.
 
 Tactic Notation "make" "simple" "indexes" "using" constr(attrlist) :=
   match goal with
